Valaig/Aig/BasicNew.lean
@@ -1,0 +1,293 @@
+module
+
+public import Std.Sat.AIG.Basic
+public import Std.Sat.AIG.CachedGates
+public import Valaig.Aig.Refs
+public import Valaig.ForStd
+
+namespace Valaig.Aig
+
+/--
+The metadata of an input in the Aig
+-/
+structure Input where
+  var : Var
+
+namespace Input
+deriving instance Hashable, DecidableEq, Repr, Inhabited for Input
+end Input
+
+/--
+The metadata of a latch in the Aig.
+
+We require all latches to have a next state defined to make it easier to define their semantics,
+even though sometimes this next state can't be known at latch construction time as they are cyclic.
+To accomodate this, the next value should initially be set to a constant, before being subsequently
+overwritten.
+
+We differ from Aiger 1.9 by requiring all latches to have a reset, meaning that all sources of
+nondeterminism in the circuit are due to inputs so are easier to reason about.
+Resets are stratified (acyclic), by requiring that the reset comes before the variable defined by
+this latch. Note that this is not compatible with the binary aiger format, so for binary aiger we
+need to reorder things to prevent this. We prefer this encoding as it is easier to reason about as
+we have an explicit order on variables.
+-/
+structure Latch where
+  var : Var
+  next : Lit
+  reset : Lit
+
+namespace Latch
+deriving instance Hashable, DecidableEq, Repr, Inhabited for Latch
+end Latch
+
+abbrev Inputs := Array Input
+abbrev Latches := Array Latch
+
+-- Switch to public by default
+end Valaig.Aig
+public section pub
+namespace Valaig.Aig
+
+/--
+An index to an input definition in the Aig input array.
+-/
+structure InputIdx where
+  ofIdx ::
+    idx : Nat
+
+namespace InputIdx
+deriving instance DecidableEq, Repr, Inhabited, BEq, ReflBEq, LawfulBEq for InputIdx
+instance : Hashable InputIdx where hash := (hash ·.idx)
+instance : LawfulHashable InputIdx where hash_eq := by simp
+end InputIdx
+
+/--
+An index to a latch definition in the Aig latch array.
+-/
+structure LatchIdx where
+  ofIdx ::
+    idx : Nat
+
+namespace LatchIdx
+deriving instance DecidableEq, Repr, Inhabited, BEq, ReflBEq, LawfulBEq for LatchIdx
+instance : Hashable LatchIdx where hash := (hash ·.idx)
+instance : LawfulHashable LatchIdx where hash_eq := by simp
+end LatchIdx
+
+/--
+An atom in the combinational aig is either an input or a latch, which is just
+a reference back to the index in the inputs or latches arrays
+-/
+inductive AtomIdx where
+| input (idx : InputIdx)
+| latch (idx : LatchIdx)
+
+namespace AtomIdx
+deriving instance Hashable, DecidableEq, Repr, Inhabited, BEq, ReflBEq, LawfulBEq for AtomIdx
+instance : LawfulHashable AtomIdx where hash_eq := by simp
+end AtomIdx
+
+/--
+An output of interest in the circuit - this is also used to represent other
+nameable nodes in the Aiger format like bad and constraint nodes
+-/
+structure Output where
+  lit : Lit
+
+namespace Output
+deriving instance Hashable, DecidableEq, Repr, Inhabited for Output
+end Output
+
+abbrev Outputs := Array Output
+
+end Aig
+
+/--
+A sequential Aig without any marked outputs. These should be stored separately
+-/
+structure Aig where
+  -- The underlying AIG
+  private aig : Std.Sat.AIG Aig.AtomIdx
+
+  -- A mapping from input indices (AtomIdx.input idx) to their definition
+  private inputs : Aig.Inputs
+
+  -- A mapping from latch indices (AtomIdx.latch idx) to their definition
+  private latches : Aig.Latches
+
+namespace Aig
+
+/--
+A representation of the node data stored for a particular variable in the Aig. For
+inputs and latches this requires a further lookup with InputIdx.get or LatchIdx.get
+-/
+inductive Node where
+  | false
+  | input (idx : InputIdx)
+  | latch (idx : LatchIdx)
+  | and (lhs rhs : Lit)
+
+namespace Node
+deriving instance Hashable, DecidableEq, Repr, Inhabited for Node
+end Node
+
+/--
+An Aig with just the constant node.
+-/
+def empty : Aig :=
+  {
+    aig := .empty,
+    inputs := #[],
+    latches := #[],
+  }
+
+/--
+The number of nodes currently allocated in the Aig
+-/
+@[local grind]
+def size (aig : Aig) : Nat :=
+  aig.aig.decls.size
+
+end Aig
+
+/-
+Variable accessors.
+-/
+
+def Var.validIn (var : Var) (aig : Aig) : Prop :=
+  var.idx < aig.size
+deriving Decidable
+
+def Lit.validIn (lit : Lit) (aig : Aig) : Prop :=
+  lit.var.validIn aig
+deriving Decidable
+
+@[always_inline]
+def Aig.get (aig : Aig) (var : Var) (valid : var.validIn aig := by grind) : Node :=
+  match aig.aig.decls[var.idx] with
+  | .false => .false
+  | .atom (.input idx) => .input idx
+  | .atom (.latch idx) => .latch idx
+  | .gate rhs0 rhs1 => .and (.ofFanin rhs0) (.ofFanin rhs1)
+
+@[inline]
+instance Aig.instGetElemVar : GetElem Aig Var Node (fun aig var => var.validIn aig) where
+  getElem aig var (h := by grind) :=
+    aig.get var h
+
+namespace Aig
+
+/-
+Input accessors.
+-/
+
+@[local simp]
+def InputIdx.validIn (idx : Aig.InputIdx) (aig : Aig) : Prop :=
+  idx.idx < aig.inputs.size
+deriving Decidable
+
+@[inline]
+def InputIdx.getVar (idx : Aig.InputIdx) (aig : Aig) (valid : idx.validIn aig := by grind) : Var :=
+  aig.inputs[idx.idx].var
+
+@[inline]
+def InputIdx.setVar (idx : Aig.InputIdx) (aig : Aig) (var : Var) (valid : idx.validIn aig := by grind) : Aig :=
+  { aig with inputs := aig.inputs.modifyMem idx.idx (by simp_all) ({ ·.val with var }) }
+
+/-
+Latch accessors.
+-/
+
+@[local simp]
+def LatchIdx.validIn (idx : Aig.LatchIdx) (aig : Aig) : Prop :=
+  idx.idx < aig.latches.size
+deriving Decidable
+
+@[inline]
+def LatchIdx.getVar (idx : Aig.LatchIdx) (aig : Aig) (valid : idx.validIn aig := by grind) : Var :=
+  aig.latches[idx.idx].var
+
+@[inline]
+def LatchIdx.setVar (idx : Aig.LatchIdx) (aig : Aig) (var : Var) (valid : idx.validIn aig := by grind) : Aig :=
+  { aig with latches := aig.latches.modifyMem idx.idx (by simp_all) ({ ·.val with var }) }
+
+@[inline]
+def LatchIdx.getNext (idx : Aig.LatchIdx) (aig : Aig) (valid : idx.validIn aig := by grind) : Lit :=
+  aig.latches[idx.idx].next
+
+@[inline]
+def LatchIdx.setNext (idx : Aig.LatchIdx) (aig : Aig) (next : Lit) (valid : idx.validIn aig := by grind) : Aig :=
+  { aig with latches := aig.latches.modifyMem idx.idx (by simp_all) ({ ·.val with next }) }
+
+@[inline]
+def LatchIdx.getReset (idx : Aig.LatchIdx) (aig : Aig) (valid : idx.validIn aig := by grind) : Lit :=
+  aig.latches[idx.idx].reset
+
+@[inline]
+def LatchIdx.setReset (idx : Aig.LatchIdx) (aig : Aig) (reset : Lit) (valid : idx.validIn aig := by grind) : Aig :=
+  { aig with latches := aig.latches.modifyMem idx.idx (by simp_all) ({ ·.val with reset }) }
+
+/-
+Generic index type that can be Var, InputIdx or LatchIdx used for proof reasoning.
+-/
+
+inductive GenericIdx where
+| node (var : Var)
+| input (idx : InputIdx)
+| latch (idx : LatchIdx)
+
+def GenericIdx.validIn (idx : GenericIdx) (aig : Aig) : Prop :=
+  match idx with
+  | node var => var.validIn aig
+  | input idx => idx.validIn aig
+  | latch idx => idx.validIn aig
+
+namespace GenericIdx
+
+variable {aig : Aig}
+attribute [local simp] validIn
+
+/-
+Lemmas to convert between specific and generic index forms.
+-/
+@[simp, grind =, grind =_] theorem iff_node (var : Var) : (node var).validIn aig ↔ var.validIn aig := by simp
+@[simp, grind =, grind =_] theorem iff_input (idx : InputIdx) : (input idx).validIn aig ↔ idx.validIn aig := by simp
+@[simp, grind =, grind =_] theorem iff_latch (idx : LatchIdx) : (latch idx).validIn aig ↔ idx.validIn aig := by simp
+
+end GenericIdx
+
+/-
+Node constructors. There is no constant node constructor as the constant node always exists, so constant
+literals can be constructed with `Lit.true`/`Lit.false`.
+-/
+
+@[inline]
+def addInput (aig : Aig) : Aig × InputIdx :=
+  let idx := .ofIdx aig.inputs.size
+  let res := aig.aig.mkAtom <| .input idx
+  let input := { var := .ofRef res.ref }
+  let inputs := aig.inputs.push input
+  let aig := { aig with aig := res.aig, inputs }
+  (aig, idx)
+
+@[inline]
+def addLatch (aig : Aig) (next reset : Lit) : Aig × LatchIdx :=
+  let idx := .ofIdx aig.latches.size
+  let res := aig.aig.mkAtom <| .latch idx
+  let latch := { var := .ofRef res.ref, next, reset }
+  let latches := aig.latches.push latch
+  let aig := { aig with aig := res.aig, latches }
+  (aig, idx)
+
+-- TODO: Currently this requires proofs that rhs0/rhs1 are valid in the aig, but after switching to
+-- buffed (and getting rid of dependent typing) this won't be needed anymore
+@[inline]
+def addAnd (aig : Aig) (rhs0 rhs1 : Lit)
+    (valid0 : rhs0.validIn aig := by grind) (valid1 : rhs1.validIn aig := by grind) : Aig × Lit :=
+  let res := aig.aig.mkAndCached ⟨rhs0.toRef valid0, rhs1.toRef valid1⟩
+  let aig := { aig with aig := res.aig }
+  (aig, .ofRef res.ref)
+
+end Valaig.Aig
+end pub
